src/proof/hashtriemap/aux.v
@@ -23,20 +23,51 @@ Section aux.
   Context `{hG: heapGS Σ, !invGS Σ, !ffi_semantics _ _}
     `{!globalsGS Σ} {go_ctx: GoContext}.
 
-  Parameter atomic_value_model : atomic.Value.t → option loc → Prop.
-  Parameter own_Value : loc -> dfrac -> option val -> iProp Σ.
+  (* Parameter atomic_value_model : atomic.Value.t → option loc → Prop. *)
+
+  (* go std library potential problem: atomic value doesnt have a nocopy embedded in it because it is older than the atomic integer types (that have the nocopy embedded) *)
+  Definition own_Value (u : loc) dq (v : interface.t) : iProp Σ :=
+    u ↦{dq} atomic.Value.mk v.
+
+  Notation "l ↦ᵥ{ dq } v" := (own_Value l dq v)
+    (at level 20, format "l  ↦ᵥ{ dq }  v").
+
+  Lemma Value_unfold l dq (v : interface.t) :
+    own_Value l dq v ⊣⊢
+    l ↦s[atomic.Value :: "v"]{dq} v.
+  Proof.
+    iSplit.
+    - iIntros "H".
+      iApply struct_fields_split in "H". iNamed "H".
+      iFrame.
+    - iIntros "Hv".
+      iApply @struct_fields_combine.
+      iFrame "Hv".
+  Qed.
 
   (* Using in place of perennial's, since perennial doesnt have std library proofs for atomic Values yet *)
-  Lemma wp_Value__Store (u: loc) (v: val) (Φ : val → iProp Σ) :
+  Lemma wp_Value__Store u v :
+    ∀ Φ,
     is_pkg_init atomic -∗
-                          (|={⊤,∅}=> ▷ ∃ old : option val,
-                                         own_Value u (DfracOwn 1) old ∗
-                                           (own_Value u (DfracOwn 1) (Some v) ={∅,⊤}=∗ Φ (# ())))
-    -∗ WP # (method_callv (ptrT.id atomic.Value.id) "Store" (# u)) (v)
-       {{ vret, Φ vret }}.
-  Proof. Admitted.
+    (|={⊤,∅}=> ▷ ∃ old, own_Value u (DfracOwn 1) old ∗ (own_Value u (DfracOwn 1) v ={∅,⊤}=∗ Φ #())) -∗
+    WP u @ (ptrT.id atomic.Value.id) @ "Store" #v {{ Φ }}.
+  Proof.
+  Admitted.
 
   #[global] Instance LoadUint32_Atomic (l:loc) : Atomic StronglyAtomic (atomic.LoadUint32 #l).
   Proof. apply _. Qed.
+
+  (* theres probably already something for this but i couldnt find it *)
+  Lemma own_slice_len_keep `{!IntoVal V} `{!IntoValTyped V t} (s: slice.t) dq (vs: list V) :
+    s ↦*{dq} vs -∗ s ↦*{dq} vs ∗
+                         ⌜length vs = sint.nat s.(slice.len_f) ∧ 0 ≤ sint.Z s.(slice.len_f)⌝.
+  Proof.
+    iIntros "Hs".
+    rewrite own_slice_unseal.
+    iDestruct "Hs" as "[Hs %Hlen]".
+    iFrame "Hs".
+    iPureIntro.
+    split; word.
+  Qed.
   
 End aux.
